src/cruft.v
@@ -1,0 +1,253 @@
+Lemma deadbranch : my_EQ iprog1 iprog2.
+Proof. 
+     unfold my_EQ.
+    unfold iprog1.
+    (* unfold iprog1 *)
+    setoid_rewrite den_iprog1_point.
+    (* process bb1 *)
+    setoid_rewrite den_bb1.
+    setoid_rewrite bind_bind.
+    setoid_rewrite bind_ret_.
+    setoid_rewrite interp_asm_SetReg.
+    setoid_rewrite bind_bind.
+    setoid_rewrite interp_asm_GetReg.
+    simpl.
+    setoid_rewrite bind_ret_.
+    (* Determine next block  *)
+    cbn.
+    setoid_rewrite bind_ret_.
+    replace (fi' _) with (f0 : fin 1) by
+      (apply unique_fin; simpl; auto).
+    setoid_rewrite bind_bind.
+    (* process bb3 *)
+    setoid_rewrite den_bb3.
+    setoid_rewrite bind_ret_.
+    setoid_rewrite bind_bind.
+    setoid_rewrite interp_asm_SetReg.
+    setoid_rewrite bind_ret_.
+    (* process input to bb4 
+        (to determine which branch jump came from)
+    *)
+    unfold from_bif, FromBifunctor_ktree_fin . cbn.
+    replace (fi' 0) with (f0 : fin 2).
+    2:{ unfold f0.  apply (symmetry jesus). }
+    (* process bb4 *)
+    setoid_rewrite den_bb4.
+    setoid_rewrite bind_bind.
+    setoid_rewrite interp_asm_GetReg.
+    setoid_rewrite bind_ret_.
+    setoid_rewrite interp_asm_SetReg. 
+    simpl.
+    (* prog1 has been processed
+       it resulted in 3 updates to the registers map *)
+
+    (* now prog2 *)
+    unfold iprog2.
+    setoid_rewrite den_iprog2_point.
+    (* process bb1' *)
+    setoid_rewrite den_bb1'.
+    setoid_rewrite bind_bind.
+    setoid_rewrite bind_ret_.
+    setoid_rewrite interp_asm_SetReg.
+    (* process bb3' *)
+    setoid_rewrite den_bb3'.
+    setoid_rewrite bind_bind.
+    setoid_rewrite bind_ret_.
+    setoid_rewrite interp_asm_SetReg.
+    simpl.
+    (* process bb4' *)
+    setoid_rewrite den_bb4'.
+    setoid_rewrite bind_bind.
+    setoid_rewrite interp_asm_GetReg.
+    setoid_rewrite bind_ret_.
+    setoid_rewrite interp_asm_SetReg.
+    simpl.
+    (* prog2 has been processed 
+        it resulted in the same 3 updates to the reigsters map *)
+    reflexivity.
+Qed.
+
+Lemma fuseBlocks : 
+    my_EQ iprog2 iprog3.
+Proof.
+    unfold my_EQ.
+    (* interpret prog2 *)
+    unfold iprog2.
+    setoid_rewrite den_iprog2_point.
+    (* interp bb1' *)
+    setoid_rewrite den_bb1'.
+    interp_asm.
+    (* interp bb3' *)
+    setoid_rewrite den_bb3'.
+    interp_asm.
+    (* interp bb4' *)
+    setoid_rewrite den_bb4'.
+    interp_asm.
+
+    (* interp prog3 *)
+    unfold iprog3.
+    (* interp bb5 *)
+    setoid_rewrite den_bb5.
+    interp_asm.
+    simpl.
+    (* both programs perform the same updates to registers *)
+    reflexivity.
+Qed.
+
+
+Lemma constantPropAndFold : my_EQ iprog3 iprog4.
+Proof.
+    unfold my_EQ.
+    (* interp prog3 *)
+    unfold iprog3.
+    unfold kprog3.
+    (* interp bb5 *)
+    setoid_rewrite den_bb5_pt.
+    interp_asm.
+    simpl.
+
+    (* interp prog4 *)
+    unfold iprog4.
+    unfold kprog4.
+    (* interp bb6 *)
+    setoid_rewrite den_bb6_pt.
+    interp_asm.
+    simpl.
+
+    (* program 3 perfroms the updates
+        (alist_add 2 5 
+        (alist_add 2 4 
+        (alist_add 1 0 [])))
+
+       program 4 performs the updates
+        (alist_add 2 5 
+        (alist_add 1 0 []))
+
+        since 
+            r2 := 5 
+        shaddows
+            r2 :=4
+        
+        these two updates are equal!
+
+        *)
+    reflexivity.
+Qed.
+
+
+Check H0. 
+        unfold EQ_registers in H0.
+        unfold eq_map in H0.
+        pose (H0 0).
+        Check mapsto_lookup.
+        Check mapsto.
+        Print lookup_def.
+        unfold lookup_default in e.
+        destruct ( lookup 0 regs1) eqn:HX; 
+        destruct ( lookup 0 regs2) eqn:HY.
+        1:{ 
+
+
+        destruct ( lookup 0 regs1) eqn:HX in e; 
+        destruct ( lookup 0 regs2) eqn:HY in e.
+        1:{ }  
+  
+
+        remember (lookup 0 regs1) as x.
+        remember (lookup 0 regs2) as y.
+        remember (lookup 0 regs1) as w in e.  
+        remember (lookup 0 regs2) as z in e.
+        destruct x ; 
+        destruct y ;
+        destruct w ;
+        destruct z ; try auto ; try constructor.
+        5:{ discriminate. }
+        destruct w'.
+        destruct (lookup 0 regs2) in e.
+
+        destruct x.
+        destruct y.
+        destruct e.
+        1:{ rewrite <- Heqx in e.  }
+        Local Transparent lookup.
+        unfold lookup.
+        
+        
+        Global Instance my_EQ_refl : Reflexive (my_EQ).
+        red.
+        intros.
+        unfold my_EQ.
+        apply ReflexiveH_Reflexive.
+        typeclasses eauto.
+        Qed.
+        
+        Global Instance my_EQ_sym : Symmetric (my_EQ).
+        red.
+        intros.
+        unfold my_EQ.
+        apply  SymmetricH_Symmetric.
+        - typeclasses eauto.
+        - exact H.
+        Qed. 
+        
+        Global Instance my_EQ_trans : Transitive (my_EQ).
+        red.
+        unfold my_EQ.
+        intros!.
+        eapply TransitiveH_Transitive.
+        - typeclasses eauto.
+        - exact H.
+        - exact H0.
+        Qed. 
+        
+        
+        Global Instance my_EQ_eqv : Equivalence (my_EQ).
+        constructor; typeclasses eauto.
+        Qed.
+
+        Lemma deadbranch : my_EQ iprog1 iprog2.
+        Proof. 
+             unfold my_EQ.
+            unfold iprog1.
+            (* unfold iprog1 *)
+            setoid_rewrite den_iprog1_point.
+            (* process bb1 *)
+            setoid_rewrite den_bb1.
+            interp_asm.
+            simpl.
+            (* Determine next block  *)
+            replace (fi' _) with (f0 : fin 1) by
+              (apply unique_fin; simpl; auto).
+            (* process bb3 *)
+            setoid_rewrite den_bb3.
+            interp_asm.
+            simpl.
+            (* process input to bb4 
+                (to determine which branch jump came from)
+            *)
+            unfold from_bif, FromBifunctor_ktree_fin . cbn.
+            replace (fi' 0) with (f0 : fin 2).
+            2:{ unfold f0.  apply (symmetry jesus). }
+            (* process bb4 *)
+            setoid_rewrite den_bb4.
+            interp_asm.
+            simpl.
+            (* prog1 has been processed
+               it resulted in 3 updates to the registers map *)
+        
+            (* now prog2 *)
+            unfold iprog2.
+            setoid_rewrite den_iprog2_point.
+            (* process bb1' *)
+            setoid_rewrite den_bb1'.
+            interp_asm.
+            (* process bb3' *)
+            setoid_rewrite den_bb3'.
+            interp_asm.
+            (* process bb4' *)
+            setoid_rewrite den_bb4'.
+            interp_asm.
+            (* prog2 has been processed 
+                it resulted in the same 3 updates to the reigsters map *)
+            reflexivity.
+        Qed.
